wip

src/drf/APredStep.v
@@ -21,17 +21,21 @@ Require Import Configuration.
 Require Import Progress.
 Require Import Behavior.
 
+Require Import AMemory.
+Require Import ALocal.
+Require Import AThread.
+
+Require Import Pred.
+
 Require Import Coq.Logic.Classical.
 
 Set Implicit Arguments.
 
 Section PredStep.
 
-  Definition te_pred := ThreadEvent.t -> Prop.
-
   Inductive pred_step (P : te_pred) lang (e:ThreadEvent.t)
              (e1 e2:Thread.t lang) : Prop :=
-  | pred_step_intro (STEP : Thread.step_allpf e e1 e2) (SAT : P e)
+  | pred_step_intro (STEP : AThread.step_allpf e e1 e2) (SAT : P e)
   .
 
   Inductive traced_step lang: list (ThreadEvent.t * Memory.t) -> (Thread.t lang) -> (Thread.t lang) -> Prop :=
@@ -41,7 +45,7 @@ Section PredStep.
       traced_step [] th0 th0
   | traced_step_step
       th0 th1 th2 hde hdm tl
-      (HD: Thread.step_allpf hde th0 th1)
+      (HD: AThread.step_allpf hde th0 th1)
       (TL: traced_step tl th1 th2)
       (MEM: hdm = th0.(Thread.memory))
     :
@@ -56,14 +60,14 @@ Section PredStep.
   | traced_step_n1_step
       th0 th1 th2 hds tle tlm
       (HD: traced_step_n1 hds th0 th1)
-      (TL: Thread.step_allpf tle th1 th2)
+      (TL: AThread.step_allpf tle th1 th2)
       (MEM: tlm = th1.(Thread.memory))
     :
       traced_step_n1 (hds++[(tle, tlm)]) th0 th2
   .
 
   Lemma traced_step_n1_one lang (th0 th1: Thread.t lang) e
-        (STEP: Thread.step_allpf e th0 th1)
+        (STEP: AThread.step_allpf e th0 th1)
     :
       traced_step_n1 [(e, th0.(Thread.memory))] th0 th1.
   Proof.
@@ -82,7 +86,7 @@ Section PredStep.
   Qed.
 
   Lemma traced_step_one lang (th0 th1: Thread.t lang) e
-        (STEP: Thread.step_allpf e th0 th1)
+        (STEP: AThread.step_allpf e th0 th1)
     :
       traced_step [(e, th0.(Thread.memory))] th0 th1.
   Proof.
@@ -137,7 +141,7 @@ Section PredStep.
     :
       exists th' th'' tr0 tr1,
         (<<STEPS0: traced_step tr0 th0 th'>>) /\
-        (<<STEP: Thread.step_allpf e th' th''>>) /\
+        (<<STEP: AThread.step_allpf e th' th''>>) /\
         (<<MEM: m = th'.(Thread.memory)>>) /\
         (<<STEPS1: traced_step tr1 th'' th1>>) /\
         (<<TRACES: tr = tr0 ++ [(e, m)] ++ tr1>>) /\
@@ -154,13 +158,13 @@ Section PredStep.
   Qed.
 
   Lemma pred_step_program_step P:
-        @pred_step P <4= @Thread.step_allpf.
+        @pred_step P <4= @AThread.step_allpf.
   Proof.
     i. inv PR. eauto.
   Qed.
 
   Lemma program_step_true_step:
-        @Thread.step_allpf <4= @pred_step (fun _ => True).
+        @AThread.step_allpf <4= @pred_step (fun _ => True).
   Proof.
     econs; eauto.
   Qed.
@@ -180,7 +184,7 @@ Section PredStep.
   Qed.
 
   Lemma thread_steps_pred_steps P lang:
-    rtc (tau (@pred_step P lang)) <2= rtc (@Thread.tau_step lang).
+    rtc (tau (@pred_step P lang)) <2= rtc (@AThread.tau_step lang).
   Proof.
     i. induction PR; eauto.
     eapply Relation_Operators.rt1n_trans; eauto.
@@ -188,7 +192,7 @@ Section PredStep.
   Qed.
 
   Lemma pred_steps_thread_steps lang:
-    rtc (@Thread.tau_step lang) <2= rtc (tau (@pred_step (fun _ => True) lang)).
+    rtc (@AThread.tau_step lang) <2= rtc (tau (@pred_step (fun _ => True) lang)).
   Proof.
     i. induction PR; eauto.
     eapply Relation_Operators.rt1n_trans; eauto.
@@ -199,7 +203,7 @@ Section PredStep.
         (STEP : rtc (tau (@pred_step P lang)) e1 e2) :
     (<<HOLD : rtc (tau (@pred_step (P /1\ Q) lang)) e1 e2>>) \/
     (<<NOT : exists e e2' e3, (<<STEPS0 : rtc (tau (@pred_step (P /1\ Q) lang)) e1 e2'>>) /\
-                              (<<STEP : Thread.step_allpf e e2' e3>>) /\
+                              (<<STEP : AThread.step_allpf e e2' e3>>) /\
                               (<<BREAKP : P e>>) /\ (<<BREAKQ : ~ Q e>>) /\
                               (<<STEPS1 : rtc (tau (@pred_step P lang)) e3 e2>>)>>).
   Proof.
@@ -214,103 +218,15 @@ Section PredStep.
     - right. repeat (econs; eauto).
   Qed.
 
-  Definition no_promise (e : ThreadEvent.t) : Prop :=
-    match e with
-    | ThreadEvent.promise _ _ _ _ _ => False
-    | _ => True
-    end.
-
-  Definition no_read_msgs (MSGS : Loc.t -> Time.t -> Prop)
-             (e : ThreadEvent.t) : Prop :=
-    match e with
-    | ThreadEvent.read loc to _ _ _ => ~ (MSGS loc to)
-    | ThreadEvent.update loc from _ _ _ _ _ _ _ => ~ (MSGS loc from)
-    | _ => True
-    end.
-
-  Definition write_not_in (MSGS : Loc.t -> Time.t -> Prop)
-             (e : ThreadEvent.t) : Prop :=
-    match e with
-    | ThreadEvent.write loc from to _ _ _ =>
-      forall t (IN: Interval.mem (from, to) t), ~ (MSGS loc t)
-    | ThreadEvent.update loc from to _ _ _ _ _ _ =>
-      forall t (IN: Interval.mem (from, to) t), ~ (MSGS loc t)
-    | ThreadEvent.promise loc from to _ _ =>
-      forall t (IN: Interval.mem (from, to) t), ~ (MSGS loc t)
-    | _ => True
-    end.
-
-  Definition no_update_on (MSGS : Loc.t -> Time.t -> Prop)
-             (e : ThreadEvent.t) : Prop :=
-    match e with
-    | ThreadEvent.update loc from to _ _ _ _ _ _ =>
-      ~ MSGS loc from
-    | _ => True
-    end.
-
-  Definition no_sc (e : ThreadEvent.t) : Prop :=
-    match e with
-    | ThreadEvent.fence _ ordw => ~ Ordering.le Ordering.seqcst ordw
-    | ThreadEvent.syscall _ => False
-    | _ => True
-    end
-  .
-
-  Definition write_in (MSGS : Loc.t -> Time.t -> Prop)
-             (e : ThreadEvent.t) : Prop :=
-    match e with
-    | ThreadEvent.write loc from to _ _ _ =>
-      forall t (IN: Interval.mem (from, to) t), (MSGS loc t)
-    | ThreadEvent.update loc from to _ _ _ _ _ _ =>
-      forall t (IN: Interval.mem (from, to) t), (MSGS loc t)
-    | _ => True
-    end.
-
-  Lemma write_not_in_mon L0 L1
-        e
-        (NOTIN: write_not_in L1 e)
-        (LE: L0 <2= L1)
-    :
-      write_not_in L0 e.
-  Proof.
-    i. unfold write_not_in in *. des_ifs.
-    - ii. eapply NOTIN; eauto.
-    - ii. eapply NOTIN; eauto.
-    - ii. eapply NOTIN; eauto.
-  Qed.
-
-  Lemma no_read_msgs_mon L0 L1
-        e
-        (NOTIN: no_read_msgs L1 e)
-        (LE: L0 <2= L1)
-    :
-      no_read_msgs L0 e.
-  Proof.
-    i. unfold no_read_msgs in *. des_ifs.
-    - ii. eapply NOTIN; eauto.
-    - ii. eapply NOTIN; eauto.
-  Qed.
-
-  Lemma no_update_on_mon L0 L1
-        e
-        (NOTIN: no_update_on L1 e)
-        (LE: L0 <2= L1)
-    :
-      no_update_on L0 e.
-  Proof.
-    i. unfold no_update_on in *. des_ifs.
-    ii. eapply NOTIN; eauto.
-  Qed.
-
   Lemma no_promise_program_step lang :
-    (@pred_step no_promise lang) <3= (@Thread.program_step lang).
+    (@pred_step no_promise lang) <3= (@AThread.program_step lang).
   Proof.
     i. inv PR. inv STEP. inv STEP0; clarify.
     inv STEP. ss.
   Qed.
 
   Lemma no_promise_program_step_rtc lang :
-    rtc (tau (@pred_step no_promise lang)) <2= rtc (tau (@Thread.program_step _)).
+    rtc (tau (@pred_step no_promise lang)) <2= rtc (tau (@AThread.program_step _)).
   Proof.
     i. induction PR.
     - refl.
@@ -349,7 +265,7 @@ Section PredStep.
     end.
 
   Lemma pf_step_promise_free_step lang:
-    @Thread.step lang true <3= @pred_step promise_free lang.
+    @AThread.step lang true <3= @pred_step promise_free lang.
   Proof.
     i. inv PR.
     - econs; eauto.
@@ -361,30 +277,13 @@ Section PredStep.
   Qed.
 
   Lemma pf_step_promise_free_step_rtc lang :
-    rtc (tau (@Thread.step _ true)) <2= rtc (tau (@pred_step promise_free lang)).
+    rtc (tau (@AThread.step _ true)) <2= rtc (tau (@pred_step promise_free lang)).
   Proof.
     i. induction PR.
     - refl.
     - econs; eauto. inv H. econs; eauto.
       eapply pf_step_promise_free_step; eauto.
   Qed.
-
-  Definition no_acq_read_msgs (MSGS : Loc.t -> Time.t -> Prop)
-             (e : ThreadEvent.t) : Prop :=
-    match e with
-    | ThreadEvent.read loc to _ _ ord =>
-      forall (SAT: MSGS loc to), ~ Ordering.le Ordering.acqrel ord
-    | ThreadEvent.update loc from _ _ _ _ _ ordr _ =>
-      forall (SAT: MSGS loc from), ~ Ordering.le Ordering.acqrel ordr
-    | _ => True
-    end
-  .
-
-  Definition is_cancel (e: ThreadEvent.t) : Prop :=
-    match e with
-    | ThreadEvent.promise _ _ _ _ Memory.op_kind_cancel => True
-    | _ => False
-    end.
 
   Definition te_rel := ThreadEvent.t -> ThreadEvent.t -> Prop.
 
@@ -396,7 +295,7 @@ Section PredStep.
         e_src e_tgt lang (th0 th1: Thread.t lang)
         (SAT: P_tgt e_tgt)
         (REL: R e_src e_tgt)
-        (STEP: Thread.step_allpf e_src th0 th1)
+        (STEP: AThread.step_allpf e_src th0 th1)
     :
       pred_step P_src e_src th0 th1.
   Proof.
@@ -405,45 +304,6 @@ Section PredStep.
 
   Definition same_machine_event e_src e_tgt :=
     ThreadEvent.get_machine_event e_src = ThreadEvent.get_machine_event e_tgt.
-
-  Definition write_not_to (MSGS : Loc.t -> Time.t -> Prop)
-             (e : ThreadEvent.t) : Prop :=
-    match e with
-    | ThreadEvent.write loc from to _ _ _ =>
-      ~ MSGS loc to
-    | ThreadEvent.update loc from to _ _ _ _ _ _ =>
-      ~ MSGS loc to
-    | ThreadEvent.promise loc from to _ _ =>
-      ~ MSGS loc to
-    | _ => True
-    end.
-
-  Definition wf_event (e: ThreadEvent.t): Prop :=
-    match e with
-    | ThreadEvent.write loc from to _ _ _ => Time.lt from to
-    | ThreadEvent.update loc from to _ _ _ _ _ _ => Time.lt from to
-    | ThreadEvent.promise loc from to _ _ => Time.lt from to
-    | _ => True
-    end.
-
-  Definition wf_time_evt (P: Loc.t -> Time.t -> Prop) (e: ThreadEvent.t) : Prop :=
-    match e with
-    | ThreadEvent.promise loc from to msg kind =>
-      (<<FROM: P loc from>>) /\ (<<TO: P loc to>>)
-    | ThreadEvent.write loc from to val released ordw =>
-      (<<FROM: P loc from>>) /\ (<<TO: P loc to>>)
-    | ThreadEvent.update loc from to valr valw releasedr releasedw ordr ordw =>
-      (<<TO: P loc to>>)
-    | _ => True
-    end.
-
-  Lemma wf_time_evt_mon P0 P1
-        (LE: P0 <2= P1)
-    :
-      wf_time_evt P0 <1= wf_time_evt P1.
-  Proof.
-    ii. unfold wf_time_evt in *. des_ifs; des; splits; eauto.
-  Qed.
 
   Lemma step_times_list_exists P lang th0 th1 e
         (STEPS: (@pred_step P lang) e th0 th1)
@@ -492,13 +352,14 @@ Section PredStep.
         i. ss. eapply List.in_or_app; eauto.
   Qed.
 
-  Definition no_acq_update_on (MSGS : Loc.t -> Time.t -> Prop)
-             (e : ThreadEvent.t) : Prop :=
-    match e with
-    | ThreadEvent.update loc from _ _ _ _ _ ordr _ =>
-      forall (SAT: MSGS loc from), ~ Ordering.le Ordering.acqrel ordr
-    | _ => True
-    end
-  .
+  Inductive opt_pred_step P lang
+    : ThreadEvent.t -> Thread.t lang -> Thread.t lang -> Prop :=
+  | step_none t: opt_pred_step P ThreadEvent.silent t t
+  | step_some
+      e t0 t1
+      (STEP: pred_step P e t0 t1)
+    :
+      opt_pred_step P e t0 t1.
+  Hint Constructors opt_pred_step.
 
 End PredStep.
