src/drf/PredStep.v
@@ -21,13 +21,13 @@ Require Import Configuration.
 Require Import Progress.
 Require Import Behavior.
 
+Require Import Pred.
+
 Require Import Coq.Logic.Classical.
 
 Set Implicit Arguments.
 
 Section PredStep.
-
-  Definition te_pred := ThreadEvent.t -> Prop.
 
   Inductive pred_step (P : te_pred) lang (e:ThreadEvent.t)
              (e1 e2:Thread.t lang) : Prop :=
@@ -214,94 +214,6 @@ Section PredStep.
     - right. repeat (econs; eauto).
   Qed.
 
-  Definition no_promise (e : ThreadEvent.t) : Prop :=
-    match e with
-    | ThreadEvent.promise _ _ _ _ _ => False
-    | _ => True
-    end.
-
-  Definition no_read_msgs (MSGS : Loc.t -> Time.t -> Prop)
-             (e : ThreadEvent.t) : Prop :=
-    match e with
-    | ThreadEvent.read loc to _ _ _ => ~ (MSGS loc to)
-    | ThreadEvent.update loc from _ _ _ _ _ _ _ => ~ (MSGS loc from)
-    | _ => True
-    end.
-
-  Definition write_not_in (MSGS : Loc.t -> Time.t -> Prop)
-             (e : ThreadEvent.t) : Prop :=
-    match e with
-    | ThreadEvent.write loc from to _ _ _ =>
-      forall t (IN: Interval.mem (from, to) t), ~ (MSGS loc t)
-    | ThreadEvent.update loc from to _ _ _ _ _ _ =>
-      forall t (IN: Interval.mem (from, to) t), ~ (MSGS loc t)
-    | ThreadEvent.promise loc from to _ _ =>
-      forall t (IN: Interval.mem (from, to) t), ~ (MSGS loc t)
-    | _ => True
-    end.
-
-  Definition no_update_on (MSGS : Loc.t -> Time.t -> Prop)
-             (e : ThreadEvent.t) : Prop :=
-    match e with
-    | ThreadEvent.update loc from to _ _ _ _ _ _ =>
-      ~ MSGS loc from
-    | _ => True
-    end.
-
-  Definition no_sc (e : ThreadEvent.t) : Prop :=
-    match e with
-    | ThreadEvent.fence _ ordw => ~ Ordering.le Ordering.seqcst ordw
-    | ThreadEvent.syscall _ => False
-    | _ => True
-    end
-  .
-
-  Definition write_in (MSGS : Loc.t -> Time.t -> Prop)
-             (e : ThreadEvent.t) : Prop :=
-    match e with
-    | ThreadEvent.write loc from to _ _ _ =>
-      forall t (IN: Interval.mem (from, to) t), (MSGS loc t)
-    | ThreadEvent.update loc from to _ _ _ _ _ _ =>
-      forall t (IN: Interval.mem (from, to) t), (MSGS loc t)
-    | _ => True
-    end.
-
-  Lemma write_not_in_mon L0 L1
-        e
-        (NOTIN: write_not_in L1 e)
-        (LE: L0 <2= L1)
-    :
-      write_not_in L0 e.
-  Proof.
-    i. unfold write_not_in in *. des_ifs.
-    - ii. eapply NOTIN; eauto.
-    - ii. eapply NOTIN; eauto.
-    - ii. eapply NOTIN; eauto.
-  Qed.
-
-  Lemma no_read_msgs_mon L0 L1
-        e
-        (NOTIN: no_read_msgs L1 e)
-        (LE: L0 <2= L1)
-    :
-      no_read_msgs L0 e.
-  Proof.
-    i. unfold no_read_msgs in *. des_ifs.
-    - ii. eapply NOTIN; eauto.
-    - ii. eapply NOTIN; eauto.
-  Qed.
-
-  Lemma no_update_on_mon L0 L1
-        e
-        (NOTIN: no_update_on L1 e)
-        (LE: L0 <2= L1)
-    :
-      no_update_on L0 e.
-  Proof.
-    i. unfold no_update_on in *. des_ifs.
-    ii. eapply NOTIN; eauto.
-  Qed.
-
   Lemma no_promise_program_step lang :
     (@pred_step no_promise lang) <3= (@Thread.program_step lang).
   Proof.
@@ -340,14 +252,6 @@ Section PredStep.
         * eauto.
   Qed.
 
-  Definition promise_free (e: ThreadEvent.t): Prop :=
-    match e with
-    | ThreadEvent.promise loc from to msg kind =>
-      (Memory.op_kind_is_lower_full kind && Message.is_released_none msg
-       || Memory.op_kind_is_cancel kind)%bool
-    | _ => True
-    end.
-
   Lemma pf_step_promise_free_step lang:
     @Thread.step lang true <3= @pred_step promise_free lang.
   Proof.
@@ -369,23 +273,6 @@ Section PredStep.
       eapply pf_step_promise_free_step; eauto.
   Qed.
 
-  Definition no_acq_read_msgs (MSGS : Loc.t -> Time.t -> Prop)
-             (e : ThreadEvent.t) : Prop :=
-    match e with
-    | ThreadEvent.read loc to _ _ ord =>
-      forall (SAT: MSGS loc to), ~ Ordering.le Ordering.acqrel ord
-    | ThreadEvent.update loc from _ _ _ _ _ ordr _ =>
-      forall (SAT: MSGS loc from), ~ Ordering.le Ordering.acqrel ordr
-    | _ => True
-    end
-  .
-
-  Definition is_cancel (e: ThreadEvent.t) : Prop :=
-    match e with
-    | ThreadEvent.promise _ _ _ _ Memory.op_kind_cancel => True
-    | _ => False
-    end.
-
   Definition te_rel := ThreadEvent.t -> ThreadEvent.t -> Prop.
 
   Definition te_pred_shift (P_src P_tgt: te_pred) (R: te_rel) :=
@@ -405,45 +292,6 @@ Section PredStep.
 
   Definition same_machine_event e_src e_tgt :=
     ThreadEvent.get_machine_event e_src = ThreadEvent.get_machine_event e_tgt.
-
-  Definition write_not_to (MSGS : Loc.t -> Time.t -> Prop)
-             (e : ThreadEvent.t) : Prop :=
-    match e with
-    | ThreadEvent.write loc from to _ _ _ =>
-      ~ MSGS loc to
-    | ThreadEvent.update loc from to _ _ _ _ _ _ =>
-      ~ MSGS loc to
-    | ThreadEvent.promise loc from to _ _ =>
-      ~ MSGS loc to
-    | _ => True
-    end.
-
-  Definition wf_event (e: ThreadEvent.t): Prop :=
-    match e with
-    | ThreadEvent.write loc from to _ _ _ => Time.lt from to
-    | ThreadEvent.update loc from to _ _ _ _ _ _ => Time.lt from to
-    | ThreadEvent.promise loc from to _ _ => Time.lt from to
-    | _ => True
-    end.
-
-  Definition wf_time_evt (P: Loc.t -> Time.t -> Prop) (e: ThreadEvent.t) : Prop :=
-    match e with
-    | ThreadEvent.promise loc from to msg kind =>
-      (<<FROM: P loc from>>) /\ (<<TO: P loc to>>)
-    | ThreadEvent.write loc from to val released ordw =>
-      (<<FROM: P loc from>>) /\ (<<TO: P loc to>>)
-    | ThreadEvent.update loc from to valr valw releasedr releasedw ordr ordw =>
-      (<<TO: P loc to>>)
-    | _ => True
-    end.
-
-  Lemma wf_time_evt_mon P0 P1
-        (LE: P0 <2= P1)
-    :
-      wf_time_evt P0 <1= wf_time_evt P1.
-  Proof.
-    ii. unfold wf_time_evt in *. des_ifs; des; splits; eauto.
-  Qed.
 
   Lemma step_times_list_exists P lang th0 th1 e
         (STEPS: (@pred_step P lang) e th0 th1)
@@ -492,13 +340,14 @@ Section PredStep.
         i. ss. eapply List.in_or_app; eauto.
   Qed.
 
-  Definition no_acq_update_on (MSGS : Loc.t -> Time.t -> Prop)
-             (e : ThreadEvent.t) : Prop :=
-    match e with
-    | ThreadEvent.update loc from _ _ _ _ _ ordr _ =>
-      forall (SAT: MSGS loc from), ~ Ordering.le Ordering.acqrel ordr
-    | _ => True
-    end
-  .
+  Inductive opt_pred_step P lang
+    : ThreadEvent.t -> Thread.t lang -> Thread.t lang -> Prop :=
+  | step_none t: opt_pred_step P ThreadEvent.silent t t
+  | step_some
+      e t0 t1
+      (STEP: pred_step P e t0 t1)
+    :
+      opt_pred_step P e t0 t1.
+  Hint Constructors opt_pred_step.
 
 End PredStep.
